\documentclass{article}
\usepackage{ifthen}
\usepackage{epsfig}
\usepackage[utf8]{inputenc}
\usepackage{newunicodechar}
  \newunicodechar{⁻}{${}^{-}$}% Superscript minus
  \newunicodechar{²}{${}^{2}$}% Superscript two
  \newunicodechar{³}{${}^{3}$}% Superscript three

\pagestyle{empty}
\begin{document}
\[ C_C(u) = \frac{\sum_{t\in T(\mathcal{G})} \pi_t(u)}{|T(\mathcal{G})|{|N(u)| \choose 2}}, \]
\pagebreak

$\pi_t(u)=|\{(v,w,t,\lambda)\in\mathcal{E}\mid v,w\in N(u)\}|$
\pagebreak

$N(u)$
\pagebreak

$u$
\pagebreak

$\tau$
\pagebreak

\[ B(\tau)=\frac{\sigma_\tau - m_\tau}{\sigma_\tau + m_\tau} \in [-1,1], \]
\pagebreak

$\sigma_\tau$
\pagebreak

$m_\tau$
\pagebreak

\[ T_{eff}(\mathcal{G})=\frac{1}{n(n-1)}\sum_{u\in V(\mathcal{G})}\sum_{v\neq u\in V(\mathcal{G})}\frac{1}{d(u,v)} \]
\pagebreak

$d(u,v)$
\pagebreak

$1/\infty=0$
\pagebreak

\[ T_{to}(u)=\frac{1}{T(\mathcal{G})}\sum_{t=1}^{T(\mathcal{G})}\frac{\sum_{v\in\mathcal{N}(u)}\phi^t_{uv}\phi^{t+1}_{uv}}{\sqrt{\sum_{v\in\mathcal{N}(u)}\phi^t_{uv}\sum_{v\in\mathcal{N}(u)}\phi^{t+1}_{uv}}}, \]
\pagebreak

$\phi^{t}_{uv}=1$
\pagebreak

$v$
\pagebreak

$t$
\pagebreak

$T_{to}(u)=1$
\pagebreak

$T_{to}(\mathcal{G})=\frac{1}{N}\sum_{u\in V}T_{to}(u)$
\pagebreak

\end{document}
